word-ram/proofs/Lax13Proofs.lean
@@ -74,6 +74,7 @@ import Lax13Proofs.Refine.Sepref.Translate
 import Lax13Proofs.Refine.Sepref.Tool
 import Lax13Proofs.Refine.Sepref.Definition
 import Lax13Proofs.Refine.Sepref.HeapAlloc
+import Lax13Proofs.Refine.Sepref.HeapCopy
 import Lax13Proofs.Refine.Sepref.HeapEO
 import Lax13Proofs.Refine.Sepref.SignaturePrep
 import Lax13Proofs.Refine.Sepref.Register
